src/util/Pftree.v
@@ -2,75 +2,79 @@ From Stdlib Require Import List.
 From Datalog.Util Require Import Tactics Fp List.
 From coqutil Require Import Tactics.fwd.
 
-Unset Elimination Schemes.
-Inductive pftree {T : Type} (P : T -> list T -> Prop) (Q : T -> Prop) : T -> Prop :=
-| pftree_leaf x :
-  Q x ->
-  pftree _ _ x
-| pftree_step x l :
-  P x l ->
-  Forall (pftree _ _) l ->
-  pftree _ _ x.
-Set Elimination Schemes.
-Hint Constructors pftree : core.
+Section __.
+  Context {T : Type}.
+  Implicit Type P : T -> list T -> Prop.
 
-Lemma pftree_ind {U : Type} (P : U -> list U -> Prop) Q R :
-  (forall x, Q x -> R x) ->
-  (forall x l,
-      P x l ->
-      Forall (pftree P Q) l ->
-      Forall R l ->
-      R x) ->
-  forall x, pftree P Q x -> R x.
-Proof.
-  intros H1 H2. fix self 2.
-  intros x Hx. invert Hx. 1: auto. eapply H2. 1,2: eassumption.
-  clear -H0 self. induction H0; eauto.
-Qed.
-Register Scheme pftree_ind as ind_nodep for pftree.
+  Unset Elimination Schemes.
+  Inductive pftree (P : T -> list T -> Prop) (Q : T -> Prop) : T -> Prop :=
+  | pftree_leaf x :
+    Q x ->
+    pftree _ _ x
+  | pftree_step x l :
+    P x l ->
+    Forall (pftree _ _) l ->
+    pftree _ _ x.
+  Set Elimination Schemes.
+  #[local] Hint Constructors pftree : core.
 
-Lemma pftree_trans {U : Type} P (x : U) Q :
-  pftree P (pftree P Q) x ->
-  pftree P Q x.
-Proof. induction 1; eauto. Qed.
+  Lemma pftree_ind P Q R :
+    (forall x, Q x -> R x) ->
+    (forall x l,
+        P x l ->
+        Forall (pftree P Q) l ->
+        Forall R l ->
+        R x) ->
+    forall x, pftree P Q x -> R x.
+  Proof.
+    intros H1 H2. fix self 2.
+    intros x Hx. invert Hx. 1: auto. eapply H2. 1,2: eassumption.
+    clear -H0 self. induction H0; eauto.
+  Qed.
+  Register Scheme pftree_ind as ind_nodep for pftree.
 
-Lemma pftree_weaken_hyp {U : Type} P (x : U) Q1 Q2 :
-  pftree P Q1 x ->
-  (forall y, Q1 y -> Q2 y) ->
-  pftree P Q2 x.
-Proof. intros H1 H2. induction H1; eauto. Qed.
+  Lemma pftree_trans P x Q :
+    pftree P (pftree P Q) x ->
+    pftree P Q x.
+  Proof. induction 1; eauto. Qed.
 
-(*TODO make this look nicer?*)
-Lemma pftree_lfp {U : Type} (P : U -> list U -> Prop) :
-  equiv (fun '(Q0, x) => pftree P Q0 x)
-    (lfp (fun Q '(Q0, x) => Q0 x \/ Q (Q0, x) \/ exists l, P x l /\ Forall (fun y => Q (Q0, y)) l)).
-Proof.
-  cbv [equiv lfp fp]. intros [Q0 x]. split; intros; fwd.
-  - apply H0. induction H; eauto.
-    right. right. exists l. split; [assumption|]. eapply Forall_impl; [eassumption|].
-    simpl. intros y. apply (H0 (_, _)).
-  - apply (H (fun '(Q, x) => _)). clear. intros [Q x]. intros [Hx| [Hx |Hx] ]; eauto.
-    fwd. eapply pftree_step; eassumption.
-Qed.
+  Lemma pftree_weaken_hyp P x Q1 Q2 :
+    pftree P Q1 x ->
+    (forall y, Q1 y -> Q2 y) ->
+    pftree P Q2 x.
+  Proof. intros H1 H2. induction H1; eauto. Qed.
 
-Lemma pftree_weaken {U : Type} P1 P2 Q (x : U) :
-  pftree P1 Q x ->
-  (forall y l, P1 y l -> P2 y l) ->
-  pftree P2 Q x.
-Proof. induction 1; eauto using Forall_impl. Qed.
+  (*TODO make this look nicer?*)
+  Lemma pftree_lfp P :
+    equiv (fun '(Q0, x) => pftree P Q0 x)
+      (lfp (fun Q '(Q0, x) => Q0 x \/ Q (Q0, x) \/ exists l, P x l /\ Forall (fun y => Q (Q0, y)) l)).
+  Proof.
+    cbv [equiv lfp fp]. intros [Q0 x]. split; intros; fwd.
+    - apply H0. induction H; eauto.
+      right. right. exists l. split; [assumption|]. eapply Forall_impl; [eassumption|].
+      simpl. intros y. apply (H0 (_, _)).
+    - apply (H (fun '(Q, x) => _)). clear. intros [Q x]. intros [Hx| [Hx |Hx] ]; eauto.
+      fwd. eapply pftree_step; eassumption.
+  Qed.
 
-Lemma pftree_equiv {U} (P1 P2 : U -> list U -> Prop) Q (x:U) :
-  (forall y l, P1 y l <-> P2 y l) ->
-  pftree P1 Q x <-> pftree P2 Q x.
-Proof.
-  intros H. split; intros Htree.
-  - eapply pftree_weaken; [exact Htree | intros y l Hyl; apply H; exact Hyl].
-  - eapply pftree_weaken; [exact Htree | intros y l Hyl; apply H; exact Hyl].
-Qed.
+  Lemma pftree_weaken (P1 P2 : T -> list T -> Prop) Q x :
+    pftree P1 Q x ->
+    (forall y l, P1 y l -> P2 y l) ->
+    pftree P2 Q x.
+  Proof. induction 1; eauto. Qed.
 
-Lemma pftree_hyp_ext P f Q1 Q2 :
-  (forall f', Q1 f' <-> Q2 f') ->
-  pftree P Q1 f <-> pftree P Q2 f.
-Proof.
-  eauto using pftree_weaken_hyp.
-Qed.
+  Lemma pftree_equiv (P1 P2 : T -> list T -> Prop) Q x :
+    (forall y l, P1 y l <-> P2 y l) ->
+    pftree P1 Q x <-> pftree P2 Q x.
+  Proof.
+    intros H. split; intros Htree.
+    - eapply pftree_weaken; [exact Htree | intros y l Hyl; apply H; exact Hyl].
+    - eapply pftree_weaken; [exact Htree | intros y l Hyl; apply H; exact Hyl].
+  Qed.
+
+  Lemma pftree_hyp_ext P f Q1 Q2 :
+    (forall f', Q1 f' <-> Q2 f') ->
+    pftree P Q1 f <-> pftree P Q2 f.
+  Proof. eauto using pftree_weaken_hyp. Qed.
+End __.
+#[export] Hint Constructors pftree : core.
